src/program_proof/wal/thread_owned.v
@@ -1,7 +1,7 @@
 From iris.proofmode Require Import tactics.
 From iris.bi.lib Require Import fractional.
 From iris.base_logic.lib Require Import iprop own.
-From Perennial.program_logic Require Import ghost_var.
+From Perennial.program_logic Require Import ghost_var_old.
 Set Default Proof Using "Type".
 
 (** resources for locking a resource but then retrieving it temporarily from a
